GripDiagnostics/Properties/Examples.lean
@@ -11,8 +11,10 @@ namespace GripDiagnostics.Properties
 open Grip
 open TermColor.Diagnostics
 
-theorem source_from_bytes_preserves_input (name : String) (bytes : ByteArray) :
-    Source.utf8Bytes (Source.fromBytes name bytes) = bytes := by
+theorem source_from_bytes_preserves_input
+    (name : String)
+    (bytes : ByteArray)
+    : Source.utf8Bytes (Source.fromBytes name bytes) = bytes := by
   rfl
 
 end GripDiagnostics.Properties
